rewrite stlc by context

coq/LC/Debruijn.v
@@ -3,7 +3,7 @@ Require Import
   Omega
   Ssreflect.ssreflect Ssreflect.ssrfun Ssreflect.ssrbool Ssreflect.eqtype
   Ssreflect.ssrnat Ssreflect.seq
-  LCAC.Relations_ext LCAC.ssrnat_ext LCAC.seq_ext.
+  LCAC.Relations_ext LCAC.ssrnat_ext LCAC.seq_ext LCAC.context.
 
 Set Implicit Arguments.
 
@@ -40,6 +40,21 @@ Fixpoint substitute n t1 t2 : term :=
         else var m
     | app t2l t2r => app (substitute n t1 t2l) (substitute n t1 t2r)
     | abs t2' => abs (substitute n.+1 t1 t2')
+  end.
+
+Fixpoint substitute_seq n ts t : term :=
+  match t with
+    | var m =>
+      if leq n m
+        then
+          (fix f ts x :=
+            if ts is t :: ts
+              then (if x is x.+1 then f ts x else shift n 0 t)
+              else var (x + n))
+          ts (m - n)
+        else var m
+    | app t1 t2 => app (substitute_seq n ts t1) (substitute_seq n ts t2)
+    | abs t' => abs (substitute_seq n.+1 ts t')
   end.
 
 Lemma shiftzero : forall n t, shift 0 n t = t.
@@ -112,6 +127,36 @@ Proof.
     - apply (shift_const_subst m t3 _ (m + n) 0); ssromega.
   - congruence.
   - by move => t1 IH m t2 t3; rewrite -addSn IH.
+Qed.
+
+Lemma substitute_seq_cons_eq :
+  forall n t ts t',
+  substitute n t (substitute_seq n.+1 ts t') = substitute_seq n (t :: ts) t'.
+Proof.
+  move => n t ts t'; elim: t' n t ts.
+  - move => /= n m t ts.
+    do !case: ifP => //=; try (do !move => ?; ssromega).
+    - move => _ H.
+      rewrite -(subnSK H).
+      elim: ts (n - m.+1) => //=.
+      - move => x; do !case: ifP => ?; try ssromega.
+        by rewrite addnS /=.
+      - move => t' ts IH; case => // {IH}.
+        symmetry.
+        rewrite -{2}(add0n m).
+        by apply shift_const_subst.
+    - move/eqnP => H _ _; subst.
+      by replace (n - n) with 0 by ssromega.
+  - by move => /= tl IHtl tr IHtr n t ts; f_equal.
+  - by move => /= t' IH n t ts; f_equal.
+Qed.
+
+Lemma substitute_seq_nil_eq : forall n t, substitute_seq n [::] t = t.
+Proof.
+  move => n t; elim: t n => /=.
+  - move => n m; case: ifP => // H; rewrite addnC subnKC //.
+  - by move => tl IHtl tr IHtr n; f_equal.
+  - by move => t H n; f_equal.
 Qed.
 
 Lemma unshift_shift_sub :
@@ -332,64 +377,87 @@ Module STLC.
 
 Inductive typ := tyvar of nat | tyfun of typ & typ.
 
-Inductive typing : seq typ -> term -> typ -> Prop :=
-  | typvar : forall ctx n ty, seqindex ctx n ty -> typing ctx (var n) ty
+Inductive typing : context typ -> term -> typ -> Prop :=
+  | typvar : forall ctx n ty, ctxindex ctx n ty -> typing ctx (var n) ty
   | typapp : forall ctx t1 t2 ty1 ty2,
     typing ctx t1 (tyfun ty1 ty2) -> typing ctx t2 ty1 ->
     typing ctx (app t1 t2) ty2
   | typabs : forall ctx t ty1 ty2,
-    typing (ty1 :: ctx) t ty2 -> typing ctx (abs t) (tyfun ty1 ty2).
+    typing (Some ty1 :: ctx) t ty2 -> typing ctx (abs t) (tyfun ty1 ty2).
 
 Lemma typvar_seqindex :
-  forall ctx n ty, typing ctx (var n) ty <-> seqindex ctx n ty.
+  forall ctx n ty, typing ctx (var n) ty <-> ctxindex ctx n ty.
 Proof.
   move => ctx n ty; split => H.
   by inversion H.
   by constructor.
 Qed.
 
-Lemma subject_shift :
-  forall t ty ctx1 ctx2 ctx3,
-  typing (ctx1 ++ ctx3) t ty ->
-  typing (ctx1 ++ ctx2 ++ ctx3) (shift (size ctx2) (size ctx1) t) ty.
+Lemma ctxleq_preserves_typing :
+  forall ctx1 ctx2 t ty,
+  ctxleq ctx1 ctx2 -> typing ctx1 t ty -> typing ctx2 t ty.
 Proof.
- elim => /=.
-  - move => n ty ctx1 ctx2 ctx3.
-    case: ifP => H; rewrite !typvar_seqindex.
-    - by rewrite -(subnKC H) {H} -addnA (addnC (n - size ctx1)) !nthopt_appr.
-    - rewrite !nthopt_appl //; ssromega.
-  - move => tl IHtl tr IHtr ty ctx1 ctx2 ctx3 H.
-    inversion H; subst; apply typapp with ty1; auto.
-  - move => t IH ty ctx1 ctx2 ctx3 H.
-    by inversion H; subst; constructor; apply (IH _ (ty1 :: ctx1)).
+  move => ctx1 ctx2 t ty H H0; move: ctx1 t ty H0 ctx2 H.
+  refine (typing_ind _ _ _ _).
+  - move => ctx2 n ty H ctx1 H0.
+    constructor; move: H0 H.
+    apply ctxleq_preserves_ctxindex.
+  - move => ctx2 tl tr tyl tyr H H0 H1 H2 ctx1 H3.
+    apply typapp with tyl; auto.
+  - move => ctx2 t tyl tyr H H0 ctx1 H1.
+    constructor; apply H0 => /=; tauto.
 Qed.
 
-Lemma subject_substitute :
-  forall ctx t1 t2 ty1 ty2 n,
-  n <= size ctx ->
-  typing (drop n ctx) t1 ty1 ->
-  typing (insert n ty1 ctx) t2 ty2 ->
-  typing ctx (substitute n t1 t2) ty2.
+Lemma subject_shift :
+  forall t ty c ctx1 ctx2,
+  typing ctx1 t ty -> typing (ctxinsert ctx2 ctx1 c) (shift (size ctx2) c t) ty.
 Proof.
-  move => ctx t1 t2; elim: t2 t1 ctx => /=.
-  - move => m t1 ctx ty1 ty2 n H H0.
-    do !(case: ifP => /=); rewrite !typvar_seqindex.
-    - move/eqnP => ? _; subst.
-      rewrite insert_nthopt_c //; case => ?; subst.
-      move: (subject_shift [::] (take m ctx) (drop m ctx) H0) => /=.
-      rewrite cat_take_drop size_takel //.
-    - move => H1 H2.
-      (have: n < m by ssromega) => {H1 H2} H1.
-      rewrite -{1}(ltn_predK H1) insert_nthopt_r //; ssromega.
-    - move => H1.
-      rewrite insert_nthopt_l //; ssromega.
-  - move => t2l IHt2l t2r IHt2r t1 ctx ty1 ty2 n H H0 H1.
-    inversion H1; subst; apply typapp with ty0.
-    - by apply IHt2l with ty1.
-    - by apply IHt2r with ty1.
-  - move => t IH t1 ctx ty1 ty2 n H H0 H1.
-    inversion H1; subst; constructor.
-    by apply (IH t1 (ty0 :: ctx) ty1 ty3).
+  move => t ty c ctx1 ctx2 H; move: ctx1 t ty H c ctx2.
+  refine (typing_ind _ _ _ _).
+  - move => /= ctx1 n ty H c ctx2.
+    case: ifP => ?; rewrite typvar_seqindex ctxnth_ctxinsert;
+      do !case: ifP => // ?; try ssromega.
+    by rewrite addnK.
+  - move => /= ctx t1 t2 ty1 ty2 H H0 H1 H2 c ctx2.
+    apply typapp with ty1; auto.
+  - move => /= ctx1 t ty1 ty2 H H0 c ctx2.
+    constructor; apply (H0 c.+1).
+Qed.
+
+Lemma subject_substitute_seq :
+  forall t ty n ctx ctx',
+  Forall (fun p => typing (drop n ctx) p.1 p.2) ctx' ->
+  typing (ctxinsert [seq Some p.2 | p <- ctx'] ctx n) t ty ->
+  typing ctx (substitute_seq n [seq p.1 | p <- ctx'] t) ty.
+Proof.
+  elim.
+  - move => /= m ty n ctx ctx'.
+    rewrite typvar_seqindex ctxnth_ctxinsert.
+    case: ifP.
+    - move/negbF; rewrite -leqNgt => H; rewrite H typvar_seqindex //.
+    - move/negbT; rewrite -leqNgt => H; rewrite H.
+      rewrite -{1 3}(subnKC H) ltn_add2l addnC.
+      move: (m - n) => {m H}.
+      elim: ctx' => //=.
+      - by move => m _; rewrite subn0; constructor.
+      - move => c' ctx' IH; case => //=.
+        - case => H _; case => H0; subst.
+          move: (subject_shift 0 (ctxinsert [::] (take n ctx) n) H).
+          rewrite /= size_ctxinsert add0n size_take minnC minKn.
+          apply ctxleq_preserves_typing.
+          (* FIXME *)
+          elim: ctx n {H IH} => [| c ctx IH].
+          - elim => //.
+          - case => /= [| n]; split; auto; apply ctxleq_refl.
+        - move => m; case => H.
+          rewrite ltnS addSn subSS.
+          apply IH.
+  - move => tl IHtl tr IHtr ty n ctx ctx' H H0.
+    inversion H0; subst => {H0}.
+    apply typapp with ty1; auto.
+  - move => /= t IH ty n ctx ctx' H H0.
+    inversion H0; subst => {H0}.
+    constructor; auto.
 Qed.
 
 Lemma subject_reduction1 :
@@ -399,8 +467,9 @@ Proof.
   refine (betared1_ind _ _ _ _ _) => //=.
   - move => t1 t2 ctx ty H.
     inversion H; subst; inversion H3; subst.
-    apply subject_substitute with ty1 => //.
-    by rewrite drop0.
+    rewrite -(substitute_seq_nil_eq 1 t1) substitute_seq_cons_eq.
+    apply (subject_substitute_seq 0 ctx [:: (t2, ty1)]) => //.
+    by rewrite /= drop0.
   - move => t1 t1' t2 H IH ctx ty H0.
     inversion H0; subst.
     by apply typapp with ty1; auto.
@@ -419,19 +488,6 @@ Proof.
     (fun t1 t2 => @subject_reduction1 ctx t1 t2 ty)).
 Qed.
 
-Lemma typing_app_ctx :
-  forall ctx ctx' t ty, typing ctx t ty -> typing (ctx ++ ctx') t ty.
-Proof.
-  move => ctx ctx'; move: ctx.
-  refine (typing_ind _ _ _ _).
-  - move => ctx n ty.
-    rewrite !typvar_seqindex.
-    by elim: n ctx => [| n IHn]; case.
-  - move => ctx t1 t2 ty1 ty2 _ H _ H0.
-    by apply typapp with ty1.
-  - by move => ctx t ty1 ty2 _ H; constructor.
-Qed.
-
 Notation SNorm t := (Acc (fun x y => betared1 y x) t).
 
 Lemma snorm_appl : forall tl tr, SNorm (app tl tr) -> SNorm tl.
@@ -441,29 +497,26 @@ Proof.
   by apply IH, H; constructor.
 Qed.
 
-Fixpoint reducible' (ctx : seq typ) (t : term) (ty : typ) : Prop :=
+Fixpoint reducible' (ctx : context typ) (t : term) (ty : typ) : Prop :=
   match ty with
     | tyvar n => SNorm t
     | tyfun ty1 ty2 => forall t1 ctx',
-        typing (ctx ++ ctx') t1 ty1 /\ reducible' (ctx ++ ctx') t1 ty1 ->
-        reducible' (ctx ++ ctx') (app t t1) ty2
+        ctxleq ctx ctx' -> typing ctx' t1 ty1 /\ reducible' ctx' t1 ty1 ->
+        reducible' ctx' (app t t1) ty2
   end.
 
 Notation reducible ctx t ty := (typing ctx t ty /\ reducible' ctx t ty).
 
 Definition neutral t := (if t is abs _ then False else True).
 
-Lemma reducible_app_ctx :
-  forall ctx1 ctx2 t ty, reducible ctx1 t ty -> reducible (ctx1 ++ ctx2) t ty.
+Lemma ctxleq_preserves_reducibility :
+  forall ctx ctx' t ty,
+  ctxleq ctx ctx' -> reducible ctx t ty -> reducible ctx' t ty.
 Proof.
-  move => ctx1 ctx2 t ty; elim: ty ctx1 ctx2 t.
-  - move => /= n ctx1 ctx2 t; case => H H0; split => //.
-    by apply typing_app_ctx.
-  - move => /= tyl IHtyl tyr IHtyr ctx1 ctx2 t1; case => H H0; split.
-    - by apply typing_app_ctx.
-    - move => t2 ctx3.
-      rewrite -catA => H1.
-      by apply H0.
+  move => ctx ctx' tl ty H; case => H0 H1; split.
+  - by apply ctxleq_preserves_typing with ctx.
+  - case: ty H H0 H1 => //= tyl tyr H H0 H1 tr ctx'' H2.
+    by apply H1, ctxleq_trans with ctx'.
 Qed.
 
 Lemma CR2' :
@@ -473,7 +526,7 @@ Proof.
   - by apply subject_reduction1 with t.
   - elim: ty ctx t t' H H1 {H0}.
     - by move => n ctx t1 t2 H; case => H0; apply H0.
-    - move => /= tyl IHtyl tyr IHtyr ctx t1 t2 H H0 t3 ctx' H1.
+    - move => /= tyl IHtyl tyr IHtyr ctx t1 t2 H H0 t3 ctx' H1 H2.
       apply IHtyr with (app t1 t3).
       - by constructor.
       - by apply H0.
@@ -500,28 +553,30 @@ Proof.
   - move => tyl; case => IHtyl1 IHtyl2 tyr;
       case => IHtyr1 IHtyr2; split => ctx t.
     - case => /= H H0.
-      have H1: typing (ctx ++ [:: tyl]) (var (size ctx)) tyl
-        by rewrite typvar_seqindex -(addn0 (size ctx))
-          nthopt_drop (drop_size_cat [:: tyl] Logic.eq_refl).
-      have H2: typing (ctx ++ [:: tyl]) (app t (var (size ctx))) tyr
-        by apply typapp with tyl => //; apply typing_app_ctx.
+      have H1: typing (ctx ++ [:: Some tyl]) (var (size ctx)) tyl
+        by rewrite typvar_seqindex ctxnth_drop' (drop_size_cat [:: Some tyl]).
+      have H2: typing (ctx ++ [:: Some tyl]) (app t (var (size ctx))) tyr
+        by apply typapp with tyl => //; move: H;
+          apply ctxleq_preserves_typing, ctxleq_appr.
       apply snorm_appl with (var (size ctx)).
-      apply IHtyr1 with (ctx ++ [:: tyl]).
+      apply IHtyr1 with (ctx ++ [:: Some tyl]).
       apply IHtyr2 => // t' H3.
       apply CR2' with (app t (var (size ctx))) => //.
       split => //.
-      apply H0, IHtyl2 => // x H4; inversion H4.
-    - move => H H0 H1 /=; split => // tr ctx' H2.
-      have H3: SNorm tr by apply IHtyl1 with (ctx ++ ctx').
-      move: tr H3 H2; refine (Acc_ind _ _) => tr _ IH H2.
-      have H3: typing (ctx ++ ctx') (app t tr) tyr.
+      apply H0.
+      - apply ctxleq_appr.
+      - apply IHtyl2 => // x H4; inversion H4.
+    - move => H H0 H1 /=; split => // tr ctx' H2 H3.
+      have H4: SNorm tr by apply IHtyl1 with ctx'.
+      move: tr H4 H2 H3; refine (Acc_ind _ _) => tr _ IH H2 H3.
+      have H4: typing ctx' (app t tr) tyr.
         apply typapp with tyl.
-        - by apply typing_app_ctx.
+        - by apply ctxleq_preserves_typing with ctx.
         - tauto.
-      apply IHtyr2 => //.
-      move => tr' H4; move: H0; inversion H4; subst => // _; split.
+      apply IHtyr2 => // tr' H5.
+      move: H0; inversion H5; subst => // _; split.
       - by apply subject_reduction1 with (app t tr).
-      - case: (H1 t1' H7); auto.
+      - case: (H1 t1' H8); auto.
       - by apply subject_reduction1 with (app t tr).
       - by apply IH => //; apply CR2' with tr.
 Qed.
@@ -557,120 +612,40 @@ Lemma apply_lemma :
 Proof.
   move => /= ctx tl tr tyl tyr; case => H H0; case => H1 H2; split.
   - by apply typapp with tyl.
-  - rewrite -(cats0 ctx).
-    apply H0.
-    by rewrite cats0; split.
+  - apply H0 => //; apply ctxleq_refl.
 Qed.
 
 Lemma abstraction_lemma :
   forall ctx t1 tyl tyr,
   typing ctx (abs t1) (tyfun tyl tyr) ->
-  (forall t2 ctx',
-   reducible (ctx ++ ctx') t2 tyl ->
-   reducible (ctx ++ ctx') (substitute 0 t2 t1) tyr) ->
+  (forall t2 ctx', ctxleq ctx ctx' ->
+   reducible ctx' t2 tyl -> reducible ctx' (substitute 0 t2 t1) tyr) ->
   reducible ctx (abs t1) (tyfun tyl tyr).
 Proof.
-  move => ctx t1 tyl tyr H H0; split => //= t2 ctx' H1.
-  suff: (reducible (ctx ++ ctx') (app (abs t1) t2) tyr) by tauto.
-  move: (snorm_subst t1 t2 (CR1 (H0 t2 ctx' H1))) (CR1 H1) => H2 H3.
-  move: t1 H2 t2 H3 H H0 H1.
-  refine (Acc_ind _ _) => t1 H H0; refine (Acc_ind _ _) => t2 H1 H2 H3 H4 H5.
+  move => ctx t1 tyl tyr H H0; split => //= t2 ctx' H1 H2.
+  suff: (reducible ctx' (app (abs t1) t2) tyr) by tauto.
+  move: (snorm_subst t1 t2 (CR1 (H0 t2 ctx' H1 H2))) (CR1 H2) => H3 H4.
+  move: t1 H3 t2 H4 H H0 H1 H2.
+  refine (Acc_ind _ _) => t1 H H0; refine (Acc_ind _ _) => t2 H1 H2 H3 H4 H5 H6.
   apply CR3 => //.
   - apply typapp with tyl.
-    - by apply typing_app_ctx.
+    - by apply ctxleq_preserves_typing with ctx.
     - tauto.
-  - move => t3 H6.
-    inversion H6; subst => {H6}.
+  - move => t3 H7.
+    inversion H7; subst => {H7}.
     - by apply H4.
-    - inversion H10; subst => {H10}.
+    - inversion H11; subst => {H11}.
       apply H0 => //.
       - by apply subject_reduction1 with (abs t1) => //; constructor.
-      - move => t'' ctx'' H6.
+      - move => t'' ctx'' H7 H9.
         apply CR2' with (substitute 0 t'' t1); auto.
         by apply subst_betared1.
     - by apply H2 => //; apply CR2' with t2.
 Qed.
 
-Fixpoint substitute_seq n ts t : term :=
-  match t with
-    | var m =>
-      if leq n m
-        then
-          (fix f ts x :=
-            if ts is t :: ts
-              then (if x is x.+1 then f ts x else shift n 0 t)
-              else var (x + n))
-          ts (m - n)
-        else var m
-    | app t1 t2 => app (substitute_seq n ts t1) (substitute_seq n ts t2)
-    | abs t' => abs (substitute_seq n.+1 ts t')
-  end.
-
-Lemma substitute_seq_cons_eq :
-  forall n t ts t',
-  substitute n t (substitute_seq n.+1 ts t') = substitute_seq n (t :: ts) t'.
-Proof.
-  move => n t ts t'; elim: t' n t ts.
-  - move => /= n m t ts.
-    do !case: ifP => //=; try (do !move => ?; ssromega).
-    - move => _ H.
-      rewrite -(subnSK H).
-      elim: ts (n - m.+1) => //=.
-      - move => x; do !case: ifP => ?; try ssromega.
-        by rewrite addnS /=.
-      - move => t' ts IH; case => // {IH}.
-        symmetry.
-        rewrite -{2}(add0n m).
-        by apply shift_const_subst.
-    - move/eqnP => H _ _; subst.
-      by replace (n - n) with 0 by ssromega.
-  - by move => /= tl IHtl tr IHtr n t ts; f_equal.
-  - by move => /= t' IH n t ts; f_equal.
-Qed.
-
-Lemma substitute_seq_nil_eq : forall n t, substitute_seq n [::] t = t.
-Proof.
-  move => n t; elim: t n => /=.
-  - move => n m; case: ifP => // H; rewrite addnC subnKC //.
-  - by move => tl IHtl tr IHtr n; f_equal.
-  - by move => t H n; f_equal.
-Qed.
-
-Lemma typing_substitute_seq :
-  forall ctx1 ctx2 ctx' t ty,
-  Forall (fun p => typing ctx2 p.1 p.2) ctx' ->
-  typing (ctx1 ++ [seq p.2 | p <- ctx'] ++ ctx2) t ty ->
-  typing (ctx1 ++ ctx2) (substitute_seq (size ctx1) [seq p.1 | p <- ctx'] t) ty.
-Proof.
-  move => ctx1 ctx2 ctx' t ty; elim: t ty ctx1 ctx2 ctx'.
-  - move => /= n ty ctx1 ctx2 ctx' H H0.
-    case: ifP => H1.
-    - move: H H0.
-      rewrite -{1}(subnKC H1).
-      elim: ctx' (n - size ctx1) => {n H1} /=.
-      - move => n _ H.
-        by rewrite addnC.
-      - move => c' ctx' IH n; case => H H0.
-        rewrite typvar_seqindex nthopt_appr.
-        case: n => //=.
-        - case => H1; subst.
-          apply (@subject_shift c'.1 c'.2 [::] ctx1 ctx2) => //.
-        - move => n H1; apply IH => //.
-          by rewrite typvar_seqindex nthopt_appr.
-    - move: H1 H0.
-      rewrite !typvar_seqindex.
-      elim: ctx1 n => // c1 ctx1 IH; case => //.
-  - move => /= tl IHtl tr IHtr ty ctx1 ctx2 ctx' H H0.
-    inversion H0; subst; apply typapp with ty1; auto.
-  - move => /= t IH ty ctx1 ctx2 ctx' H H0.
-    inversion H0; subst => {H0}.
-    constructor.
-    by apply (IH ty2 (ty1 :: ctx1) ctx2 ctx').
-Qed.
-
 Lemma reduce_lemma :
   forall ctx (ctx' : seq (term * typ)) t ty,
-  typing ([seq p.2 | p <- ctx'] ++ ctx) t ty ->
+  typing ([seq Some p.2 | p <- ctx'] ++ ctx) t ty ->
   Forall (fun p => reducible ctx p.1 p.2) ctx' ->
   reducible ctx (substitute_seq 0 [seq p.1 | p <- ctx'] t) ty.
 Proof.
@@ -695,23 +670,25 @@ Proof.
     inversion H; subst => {H}.
     move: (IHtl (tyfun ty1 ty) ctx ctx'); case => //= H1 H2; split.
     - apply typapp with ty1 => //.
-      apply (typing_substitute_seq [::]) => //.
-      by move: H0; apply Forall_impl => p; case.
-    - rewrite -(cats0 ctx); apply H2; rewrite cats0.
-      by apply IHtr.
+      apply subject_substitute_seq => //=.
+      by rewrite drop0; move: H0; apply Forall_impl => p; case.
+    - apply H2.
+      - apply ctxleq_refl.
+      - by apply IHtr.
   - move => t IHt ty ctx ctx' H H0.
     inversion H; subst => {H} /=.
     apply abstraction_lemma.
-    - apply (@typing_substitute_seq [::] ctx ctx' (abs t)) => //=.
-      - by move: H0; apply Forall_impl => p; case.
-      - by constructor.
-    - move => t2 ctx2 H.
+    - constructor.
+      apply subject_substitute_seq => //.
+      by rewrite /= drop0; move: H0; apply Forall_impl => p; case.
+    - move => t2 ctx2 H H1.
       rewrite substitute_seq_cons_eq -/[seq p.1 | p <- (t2, ty1) :: ctx'].
-      apply IHt.
-      - by rewrite catA; apply typing_app_ctx => /=.
+      apply IHt => /=.
+      - move: H3; apply ctxleq_preserves_typing.
+        move: H; apply (ctxleq_appl (Some ty1 :: _)).
       - split => //.
         move: H0; apply Forall_impl => p.
-        apply reducible_app_ctx.
+        by apply ctxleq_preserves_reducibility.
 Qed.
 
 Theorem typed_term_is_snorm : forall ctx t ty, typing ctx t ty -> SNorm t.
