coq/context.v
@@ -9,16 +9,15 @@ Section context.
 
 Variable (A : Type).
 
-Notation context := (seq (option A)).
+Definition context := (seq (option A)).
 
 (* ctxleq *)
 
 Fixpoint ctxleq (xs ys : context) : Prop :=
   match xs, ys with
-    | _, [::] => True
-    | [::], y :: ys => y = None /\ ctxleq [::] ys
-    | x :: xs, y :: ys =>
-      (x = y \/ y = None) /\ ctxleq xs ys
+    | [::], _ => True
+    | x :: xs, [::] => x = None /\ ctxleq xs [::]
+    | x :: xs, y :: ys => (x = y \/ x = None) /\ ctxleq xs ys
   end.
 
 Theorem ctxleq_refl : forall xs, ctxleq xs xs.
@@ -29,29 +28,29 @@ Qed.
 Theorem ctxleq_trans :
   forall xs ys zs, ctxleq xs ys -> ctxleq ys zs -> ctxleq xs zs.
 Proof.
-  elim => /=.
-  - elim => // y ys IH; case => //= z zs.
-    case => H H0; case => H1 H2; split.
-    - by case: H1 => H1; subst.
-    - by apply IH.
-  - move => x xs IH; case => /=.
-    - move => {IH} zs _.
-      elim: zs {x xs} (x :: xs) => //=.
-      - case => //.
-      - move => z zs IH; case => // x xs; case => H H0; subst; split.
-        - tauto.
-        - by apply IH.
-    - move => y ys; case => //= z zs; case => H H0; case => H1 H2; split.
-      - case: H; case: H1 => H H1; subst; tauto.
-      - by apply IH with ys.
+  elim => // x xs IH; case => /= [| y ys].
+  - case => // z zs; case => H H0 _; subst; split; auto.
+    apply IH with [::] => //.
+  - case => //.
+    - case; case => H H0; case => H1 H2; subst; split; auto;
+        apply IH with ys => //.
+    - move => z zs.
+      case; case => H H0; case; case => H1 H2; subst; split; auto;
+        apply IH with ys => //.
 Qed.
 
-Theorem ctxleq_nil : forall xs, ctxleq xs [::].
+Theorem ctxleq_nil : forall xs, ctxleq [::] xs.
 Proof.
   by case.
 Qed.
 
-Theorem ctxleq_appr : forall xs ys, ctxleq (xs ++ ys) xs.
+Theorem ctxleq_appl :
+  forall xs ys zs, ctxleq ys zs -> ctxleq (xs ++ ys) (xs ++ zs).
+Proof.
+  elim => //=; auto.
+Qed.
+
+Theorem ctxleq_appr : forall xs ys, ctxleq xs (xs ++ ys).
 Proof.
   move => xs ys; elim: xs.
   - apply ctxleq_nil.
@@ -153,15 +152,15 @@ Notation ctxindex xs n x := (Some x = ctxnth xs n).
 
 Theorem ctxleq_preserves_ctxindex :
   forall xs ys n a,
-  ctxleq xs ys -> ctxindex ys n a -> ctxindex xs n a.
+  ctxleq xs ys -> ctxindex xs n a -> ctxindex ys n a.
 Proof.
-  elim => [| x xs IH]; case => // y ys; case => /= [| n] a.
+  elim => // x xs IH; case => [| y ys]; case => /= [| n] a.
   - by case => H; subst.
   - case => H; subst => H H0; apply False_ind.
-    elim: ys n H H0 => //= y ys IH; case.
+    elim: xs n H H0 {IH} => // x xs IH; case => /= [| n].
     - by case => H; subst.
-    - move => n; case => H; subst; apply IH.
-  - by case; case => H; subst.
+    - case => H; subst; apply IH.
+  - by case; case => H H0; subst.
   - case => _; apply IH.
 Qed.
 
