coq/seq_ext.v
@@ -11,11 +11,6 @@ Section Seq.
 
 Variable (A : Type).
 
-Function insert (n : nat) (a : A) (xs : seq A) :=
-  if n is n.+1
-    then (if xs is x :: xs then x :: insert n a xs else [:: a])
-    else a :: xs.
-
 Fixpoint nthopt (xs : seq A) n :=
   if xs is x :: xs
     then (if n is n.+1 then nthopt xs n else Some x)
@@ -51,69 +46,9 @@ Proof.
   by move => n xs; rewrite drop_take_distr -(addn0 n) subnDl take0.
 Qed.
 
-(* nthopt *)
-
-Theorem nthopt_drop : forall xs n m, nthopt xs (n + m) = nthopt (drop n xs) m.
+Theorem size_take : forall n (xs : seq A), size (take n xs) = minn n (size xs).
 Proof.
-  by elim => // x xs IH; case.
-Qed.
-
-Theorem nthopt_drop' : forall xs n, nthopt xs n = nthopt (drop n xs) 0.
-Proof.
-  by move => xs n; rewrite -{1}(addn0 n) nthopt_drop.
-Qed.
-
-Theorem nthopt_take0 : forall xs n m, m <= n -> nthopt (take m xs) n = None.
-Proof.
-  by elim => // x xs IH n; case => // m; case: n => //= n H; rewrite IH.
-Qed.
-
-Theorem nthopt_take1 :
-  forall xs n m, n < m -> nthopt (take m xs) n = nthopt xs n.
-Proof.
-  by elim => // x xs IH n; case => // m; case: n => //= n H; rewrite IH.
-Qed.
-
-Theorem nthopt_appl :
-  forall xs ys n, n < size xs -> nthopt (xs ++ ys) n = nthopt xs n.
-Proof.
-  by move => xs ys; elim: xs => // x xs IH; case.
-Qed.
-
-Theorem nthopt_appr :
-  forall xs ys n, nthopt (xs ++ ys) (size xs + n) = nthopt ys n.
-Proof.
-  by elim.
-Qed.
-
-(* insert *)
-
-Theorem insert_eq : forall n a xs, insert n a xs = take n xs ++ a :: drop n xs.
-Proof.
-  move => n a; elim: n => [| n IH].
-  - by move => xs; rewrite take0 drop0.
-  - by case => //= x xs; f_equal.
-Qed.
-
-Theorem insert_nthopt_l :
-  forall m n a xs,
-  m < n -> m < size xs -> nthopt (insert n a xs) m = nthopt xs m.
-Proof.
-  move => m n a xs; elim: xs n m => // x xs IH; case => // n; case => //= m.
-  rewrite !ltnS; apply IH.
-Qed.
-
-Theorem insert_nthopt_c :
-  forall n a xs, n <= size xs -> nthopt (insert n a xs) n = Some a.
-Proof.
-  by move => n a; elim: n => // n IH; case.
-Qed.
-
-Theorem insert_nthopt_r :
-  forall m n a xs, n <= m -> nthopt (insert n a xs) m.+1 = nthopt xs m.
-Proof.
-  move => m n a; elim: m n => [| m IH];
-    case => // n; case => //= _ xs; apply IH.
+  by elim => [| n IH]; case => //= x xs; rewrite IH minnSS.
 Qed.
 
 (* Forall *)
@@ -126,5 +61,3 @@ Proof.
 Qed.
 
 End Seq.
-
-Notation seqindex xs n x := (Some x = nthopt xs n).
